theories/L2d_flattenedApp/wNorm.v
@@ -1,5 +1,4 @@
 
-
 Require Import Coq.Lists.List.
 Require Import Coq.Strings.String.
 Require Import Coq.Strings.Ascii.
